---
title: "Multiple Testing Project"
output: pdf_document
---

# 2.2 P-value

## 1. Distribution of the p-value under the null

**1.1 Show that for any $\alpha$, $c_{\alpha} = F_{H}^{-1}(1 - \alpha)$**

We know that $\alpha = 1 - F_{H}(c_{\alpha})$ from the definition of $c_{\alpha}$.

$\alpha = 1 - F_{H}(c_{\alpha})$

$\alpha - 1 = - F_{H}(c_{\alpha})$

$-(\alpha - 1) = F_{H}(c_{\alpha})$

$1 - \alpha = F_{H}(c_{\alpha})$

$F^{-1}_{H}(1 - \alpha) = c_{\alpha}$

$c_{\alpha} = F^{-1}_{H}(1 - \alpha)$

Q.E.D.

**1.2 Show that the p-value of the test, as a function of the data X used, is given by $p(\textbf{X}) = 1 - F_{H}(T(\textbf{X}))$.**

The p-value is defined as $p-value = inf\{\alpha : T(X) \in R_{\alpha}\}$

Which is to say that the p-value is the *smallest* $\alpha$ for which $T(X)$ is in the region $R_{\alpha}$ of the probability distribution $P_{H}$

So the p-value is an instance of $\alpha$, which is defined as $\alpha = 1 - F_{H}(c_{\alpha})$ where $c_{\alpha}$ is chosen so that the equation is true. Therefore, if we replace $c_{\alpha}$ with our test statistic $T(\textbf{X})$, we get a $p(\textbf{X}) = 1 - F_{H}(\textbf{X})$.

This matters because it highlights that the choice of $\alpha$ sets the minimum p-value for $\textbf{X}$ as $p(\textbf{X})$ such that one rejects the hypothesis that X is from the same distribution as Y when $T(\textbf{X}) > c_{\alpha}$.

From the previous question we know, 
$F_{H}(c_{\alpha}) = 1 - \alpha$

$F_{H}(c_{\alpha}) = 1 - P_{H}[T(\textbf{X}) > c_{\alpha}]$

$P_{H}[T(\textbf{X}) > c_{\alpha}] = 1 - F_{H}(c_{\alpha})$

$P_{H}[T(\textbf{X}) > \textbf{x}] = 1 - F_{H}(\textbf{X})$

$p(\textbf{X}) = 1 - F_{H}(\textbf{X})$


**1.3 Show that for any univariate random variable $y$ with continuous distribution function $F$, the random variables $F(y)$ and $1 - F(y)$ follow the uniform distribution.**

We know that the CDF of a uniform distribution is as follows,

$F(y)$$\begin{cases} 
      0 & y\leq a \\
      \frac{y - a}{b - a} & a\leq y\leq b \\
      1 & y \leq b  
   \end{cases}$

$1 - F(y)$$\begin{cases} 
      1 & y\leq a \\
      1 - \frac{y - a}{b - a} & a\leq y\leq b \\
      0 & y \leq b  
   \end{cases}$

$1 - F(y)$$\begin{cases} 
      1 & y\leq a \\
      \frac{b - y}{b - a} & a\leq y\leq b \\
      0 & y \leq b  
   \end{cases}$

$1 - F(y)$$\begin{cases} 
      1 & y\leq a \\
      \frac{y - b}{a - b} & b\leq y\leq a \\
      0 & y \leq b  
   \end{cases}$

which is the CDF for another unifrom random distribution.

**1.4 Using the above results, show that the p-value follows the uniform distribution under H.**

$\alpha = 1 - F_{H}(c_{\alpha})$

If $F_{H}(c_{\alpha})$ follows a uniform distribution, $1 - F_{H}(c_{\alpha})$ does too, as proven in the previous exercise. 


